src/lowparse/LowParse.Writers.Instances.fsti
@@ -51,6 +51,20 @@ val valid_rewrite_parse_synth_gen
   ))
 : Tot (valid_rewrite_t p1 p2 (fun _ -> True) f2)
 
+val valid_rewrite_parse_synth_gen_recip
+  (p1: parser)
+  (p2: parser)
+  (f2: Parser?.t p1 -> GTot (Parser?.t p2))
+  (f1: Parser?.t p2 -> GTot (Parser?.t p1))
+  (sq: squash (
+    LP.synth_injective f2 /\
+    LP.synth_inverse f2 f1 /\
+    get_parser_kind p2 == get_parser_kind p1 /\
+    get_parser p2 == LP.coerce (LP.parser (get_parser_kind p2) (Parser?.t p2)) (get_parser p1 `LP.parse_synth` f2) /\
+    get_serializer p2 == LP.coerce (LP.serializer (get_parser p2)) (LP.serialize_synth (get_parser p1) f2 (get_serializer p1) f1 ())
+  ))
+: Tot (valid_rewrite_t p2 p1 (fun _ -> True) f1)
+
 let valid_rewrite_parse_synth
   (p1: parser)
   (#t2: Type)
@@ -63,7 +77,7 @@ let valid_rewrite_parse_synth
 : Tot (valid_rewrite_t p1 (parse_synth p1 f2 f1) (fun _ -> True) f2)
 = valid_rewrite_parse_synth_gen _ _ _ f1 ()
 
-val valid_rewrite_parse_synth_recip
+let valid_rewrite_parse_synth_recip
   (p1: parser)
   (#t2: Type)
   (f2: Parser?.t p1 -> GTot t2)
@@ -73,6 +87,7 @@ val valid_rewrite_parse_synth_recip
     LP.synth_inverse f2 f1
   ))
 : Tot (valid_rewrite_t (parse_synth p1 f2 f1) p1 (fun _ -> True) f1)
+= valid_rewrite_parse_synth_gen_recip _ _ f2 _ ()
 
 module U32 = FStar.UInt32
 
